progress on proving memory safety

code/experimental/rsa/Hacl.Impl.MGF.fst
@@ -25,58 +25,56 @@ assume val hash_sha256:
 //let hash_sha256 #len mHash clen m = SHA2_256.hash mHash m clen
 
 (* Mask Generation Function *)
-val mgf_:
-    #accLen:size_nat -> #stLen:size_nat ->
+val mgf_sha256_:
     count_max:size_t ->
-    mgfseed:lbytes (v hLen) ->
-    aaccLen:size_t{v aaccLen == accLen /\  accLen = v hLen * v count_max} ->
-    sstLen:size_t{v sstLen == stLen /\ stLen = v hLen + 4 + 4 + v hLen + accLen} -> st:lbytes stLen ->
+    accLen:size_t{v accLen = v hLen * v count_max} ->
+    stLen:size_t{v stLen = 4 + 2 * v hLen + v accLen} -> st:lbytes (v stLen) ->
     counter:size_t{v counter <= v count_max} -> Stack unit
-    (requires (fun h -> live h mgfseed /\ live h st /\ disjoint st mgfseed))
+    (requires (fun h -> live h st))
     (ensures (fun h0 _ h1 -> preserves_live h0 h1 /\ modifies1 st h0 h1))
-
-#reset-options "--z3rlimit 50 --max_fuel 0 --max_ifuel 0"
+    #reset-options "--z3rlimit 50 --max_fuel 0 --max_ifuel 0"
     [@"c_inline"]
-let rec mgf_ #accLen #stLen count_max mgfseed aaccLen sstLen st counter =
+let rec mgf_sha256_ count_max accLen stLen st counter =
   if (counter <. count_max) then begin
-     let mgfseed_counter = Buffer.sub #uint8 #stLen #(v hLen + 4) st (size 0) (add #SIZE hLen (size 4)) in
-     let c = Buffer.sub #uint8 #stLen #4 st (add #SIZE hLen (size 4)) (size 4) in
-     let mHash = Buffer.sub #uint8 #stLen #(v hLen) st (add #SIZE hLen (size 8)) hLen in
-     let acc = Buffer.sub #uint8 #stLen #accLen st (add #SIZE (add #SIZE hLen (size 8)) hLen) aaccLen in
+     let mgfseed_counter_len = add #SIZE hLen (size 4) in
+     let mgfseed_counter = Buffer.sub #uint8 #(v stLen) #(v mgfseed_counter_len) st (size 0) mgfseed_counter_len in
+     let mHash = Buffer.sub #uint8 #(v stLen) #(v hLen) st mgfseed_counter_len hLen in
+     let acc = Buffer.sub #uint8 #(v stLen) #(v accLen) st (add #SIZE mgfseed_counter_len hLen) accLen in
+     let c = Buffer.sub #uint8 #(v mgfseed_counter_len) #4 mgfseed_counter hLen (size 4) in
      c.(size 0) <- to_u8 #U32 (size_to_uint32 counter >>. u32 24);
      c.(size 1) <- to_u8 #U32 (size_to_uint32 counter >>. u32 16);
      c.(size 2) <- to_u8 #U32 (size_to_uint32 counter >>. u32 8);
      c.(size 3) <- to_u8 #U32 (size_to_uint32 counter);
 
-     let mgfseed_counter_ = Buffer.sub #uint8 #(v hLen + 4) #4 mgfseed_counter hLen (size 4) in
-     copy (size 4) c mgfseed_counter_;
-     hash_sha256 mHash (add #SIZE hLen (size 4)) mgfseed_counter;
-     let acc_ = Buffer.sub #uint8 #accLen #(v hLen) acc (mul #SIZE hLen counter) hLen in
-     copy hLen mHash acc_;
-     mgf_ #accLen #stLen count_max mgfseed aaccLen sstLen st (size_incr counter)
+     hash_sha256 mHash mgfseed_counter_len mgfseed_counter;
+     let acc' = Buffer.sub #uint8 #(v accLen) #(v hLen) acc (mul #SIZE hLen counter) hLen in
+     copy hLen mHash acc';
+     mgf_sha256_ count_max accLen stLen st (size_incr counter)
   end
 
 val mgf_sha256:
     #len:size_nat ->
     mgfseed:lbytes (v hLen) ->
-    clen:size_t{v clen == len /\ 0 < len /\ 8 + 2 * v hLen + v hLen * v (blocks clen hLen) < max_size_t} ->
+    clen:size_t{v clen == len /\ 0 < len /\ 4 + 2 * v hLen + v hLen * v (blocks clen hLen) < max_size_t} ->
     res:lbytes len -> Stack unit
     (requires (fun h -> live h mgfseed /\ live h res /\ disjoint res mgfseed))
     (ensures (fun h0 _ h1 -> preserves_live h0 h1 /\ modifies1 res h0 h1))
-    [@"c_inline"]	
+    [@"c_inline"]
 let mgf_sha256 #len mgfseed clen res =
     let count_max = blocks clen hLen in
     let accLen = mul #SIZE hLen count_max in
-    let stLen = add #SIZE (add #SIZE (add #SIZE hLen (size 8)) hLen) accLen in
+    let mgfseed_counter_len = add #SIZE hLen (size 4) in
+    let stLen = add #SIZE (add #SIZE mgfseed_counter_len hLen) accLen in
     
     alloc #uint8 #unit #(v stLen) stLen (u8 0) [BufItem mgfseed] [BufItem res]
     (fun h0 _ h1 -> True)
     (fun st ->
-       let mgfseed_counter = Buffer.sub #uint8 #(v stLen) #(v hLen + 4) st (size 0) (add #SIZE hLen (size 4)) in
-       let acc = Buffer.sub #uint8 #(v stLen) #(v accLen) st (add #SIZE (add #SIZE hLen (size 8)) hLen) accLen in
-       let mgfseed_counter_ = Buffer.sub #uint8 #(v hLen + 4) #(v hLen) mgfseed_counter (size 0) hLen in
-       copy hLen mgfseed mgfseed_counter_;
-       mgf_ #(v accLen) #(v stLen) count_max mgfseed accLen stLen st (size 0);
-       let acc_ = Buffer.sub #uint8 #(v accLen) #len acc (size 0) clen in
-       copy clen acc_ res
+       let mgfseed_counter = Buffer.sub #uint8 #(v stLen) #(v mgfseed_counter_len) st (size 0) mgfseed_counter_len in
+       let mgfseed_counter' = Buffer.sub #uint8 #(v mgfseed_counter_len) #(v hLen) mgfseed_counter (size 0) hLen in
+       copy hLen mgfseed mgfseed_counter';
+       //let mHash = Buffer.sub #uint8 #(v stLen) #(v hLen) st mgfseed_counter_len hLen in
+       let acc = Buffer.sub #uint8 #(v stLen) #(v accLen) st (add #SIZE mgfseed_counter_len hLen) accLen in
+       mgf_sha256_ count_max accLen stLen st (size 0);
+       let acc' = Buffer.sub #uint8 #(v accLen) #len acc (size 0) clen in
+       copy clen acc' res
     )
