code/experimental/rsa/Hacl.Impl.RSA.fst
@@ -26,46 +26,8 @@ val xor_bytes:
     b2:lbytes len -> Stack unit
     (requires (fun h -> live h b1 /\ live h b2))
     (ensures (fun h0 _ h1 -> preserves_live h0 h1 /\ modifies1 b1 h0 h1))
+    [@"c_inline"]
 let xor_bytes #len clen b1 b2 = map2 #uint8 #uint8 #len clen (fun x y -> logxor #U8 x y) b1 b2
-
-val pss_encode_in:
-    #sLen:size_nat -> #msgLen:size_nat -> #emLen:size_nat -> #stLen:size_nat ->
-    ssLen:size_t{v ssLen == sLen /\ sLen + v hLen + 8 < max_size_t} -> salt:lbytes sLen ->
-    mmsgLen:size_t{v mmsgLen == msgLen} -> msg:lbytes msgLen ->
-    eemLen:size_t{v eemLen == emLen /\ emLen - sLen - v hLen - 2 >= 0} ->
-    m1_size:size_t{v m1_size = 8 + v hLen + sLen} -> 
-    db_size:size_t{v db_size = emLen - v hLen - 1} ->
-    sstLen:size_t{v sstLen == stLen /\ stLen = v hLen + v m1_size + v hLen + v db_size + v db_size} -> st:lbytes stLen -> Stack unit
-    (requires (fun h -> live h salt /\ live h msg /\ live h st /\ disjoint st msg /\ disjoint st salt /\ disjoint msg salt))
-    (ensures (fun h0 _ h1 -> preserves_live h0 h1 /\ modifies1 st h0 h1))
-
-#reset-options "--z3rlimit 50 --max_fuel 0 --max_ifuel 0"
-[@ "substitute"]
-let pss_encode_in #sLen #msgLen #emLen #stLen ssLen salt mmsgLen msg eemLen m1_size db_size sstLen st =
-    let mHash = Buffer.sub #uint8 #stLen #(v hLen) st (size 0) hLen in
-    disjoint_sub_lemma1 st msg (size 0) hLen;
-    hash_sha256 mHash mmsgLen msg;
-    
-    let m1 = Buffer.sub #uint8 #stLen #(v m1_size) st hLen m1_size in
-    let m1_ = Buffer.sub #uint8 #(v m1_size) #(v hLen) m1 (size 8) hLen in
-    copy hLen mHash m1_;
-    let m1_ = Buffer.sub #uint8 #(v m1_size) #sLen m1 (add #SIZE (size 8) hLen) ssLen in
-    copy ssLen salt m1_;
-    
-    let m1Hash = Buffer.sub #uint8 #stLen #(v hLen) st (add #SIZE hLen m1_size) hLen in
-    hash_sha256 m1Hash m1_size m1;
-    
-    let db = Buffer.sub #uint8 #stLen #(v db_size) st (add #SIZE (add #SIZE hLen m1_size) hLen) db_size in
-    let last_before_salt = sub #SIZE (sub #SIZE db_size ssLen) (size 1) in
-    db.(last_before_salt) <- u8 1;
-    let db_ = Buffer.sub #uint8 #(v db_size) #sLen db (size_incr last_before_salt) ssLen in
-    copy ssLen salt db_;
-    
-    let dbMask = Buffer.sub #uint8 #stLen #(v db_size) st (add #SIZE (add #SIZE (add #SIZE hLen m1_size) hLen) db_size) db_size in
-    assume (8 + 2 * v hLen + v hLen * v (blocks db_size hLen) < max_size_t);
-    mgf_sha256 m1Hash db_size dbMask;
-    xor_bytes db_size db dbMask
-
   
 val pss_encode_:
     #sLen:size_nat -> #msgLen:size_nat -> #emLen:size_nat ->
@@ -74,27 +36,48 @@ val pss_encode_:
     mmsgLen:size_t{v mmsgLen == msgLen} -> msg:lbytes msgLen ->
     eemLen:size_t{v eemLen == emLen /\  emLen - sLen - v hLen - 2 >= 0} ->
     em:lbytes emLen -> Stack unit
-    (requires (fun h -> live h salt /\ live h msg /\ live h em /\ disjoint msg salt /\ disjoint em msg /\ disjoint em salt))
+    (requires (fun h -> live h salt /\ live h msg /\ live h em /\ 
+	              disjoint msg salt /\ disjoint em msg /\ disjoint em salt))
     (ensures (fun h0 _ h1 -> preserves_live h0 h1 /\ modifies1 em h0 h1))
-
-#reset-options "--z3rlimit 50 --max_fuel 0 --max_ifuel 0"
-
+    #reset-options "--z3rlimit 150 --max_fuel 0 --max_ifuel 0"
+    [@"c_inline"]
 let pss_encode_ #sLen #msgLen #emLen ssLen salt mmsgLen msg eemLen em =
-    let m1_size = add #SIZE (add #SIZE (size 8) hLen) ssLen in
-    let db_size = sub #SIZE (sub #SIZE eemLen hLen) (size 1) in
-    assume (v hLen + v m1_size + v hLen + v db_size + v db_size < max_size_t);
-    let stLen = add #SIZE (add #SIZE (add #SIZE (add #SIZE hLen m1_size) hLen) db_size) db_size in
+    let m1_size:size_t = add #SIZE (add #SIZE (size 8) hLen) ssLen in
+    let db_size:size_t = sub #SIZE (sub #SIZE eemLen hLen) (size 1) in
+    
+    assume (sLen + v hLen + 8 + 2 * emLen < max_size_t);
+    assume (4 + 2 * v hLen + v hLen * v (blocks db_size hLen) < max_size_t);
+    let stLen:size_t = add #SIZE (add #SIZE (add #SIZE (add #SIZE hLen m1_size) hLen) db_size) db_size in
 
     alloc #uint8 #unit #(v stLen) stLen (u8 0) [BufItem salt; BufItem msg] [BufItem em]
     (fun h0 _ h1 -> True)
     (fun st ->
-       pss_encode_in #sLen #msgLen #emLen #(v stLen) ssLen salt mmsgLen msg eemLen m1_size db_size stLen st;
-       let db = Buffer.sub #uint8 #(v stLen) #(v db_size) st (add #SIZE (add #SIZE hLen m1_size) hLen) db_size in
-       let em_ = Buffer.sub #uint8 #emLen #(v db_size) em (size 0) db_size in
-       copy db_size db em_;
-       let em_ = Buffer.sub #uint8 #emLen #(v hLen) em db_size hLen in
+       let mHash = Buffer.sub #uint8 #(v stLen) #(v hLen) st (size 0) hLen in
+       let m1 = Buffer.sub #uint8 #(v stLen) #(v m1_size) st hLen m1_size in
        let m1Hash = Buffer.sub #uint8 #(v stLen) #(v hLen) st (add #SIZE hLen m1_size) hLen in
-       copy hLen m1Hash em_;
+       let db = Buffer.sub #uint8 #(v stLen) #(v db_size) st (add #SIZE (add #SIZE hLen m1_size) hLen) db_size in
+       let dbMask = Buffer.sub #uint8 #(v stLen) #(v db_size) st (add #SIZE (add #SIZE (add #SIZE hLen m1_size) hLen) db_size) db_size in
+       disjoint_sub_lemma1 st msg (size 0) hLen;
+       hash_sha256 mHash mmsgLen msg;
+    
+       let m1' = Buffer.sub #uint8 #(v m1_size) #(v hLen) m1 (size 8) hLen in
+       copy hLen mHash m1';
+       let m1' = Buffer.sub #uint8 #(v m1_size) #sLen m1 (add #SIZE (size 8) hLen) ssLen in
+       copy ssLen salt m1';
+       hash_sha256 m1Hash m1_size m1;
+       
+       let last_before_salt = sub #SIZE (sub #SIZE db_size ssLen) (size 1) in
+       db.(last_before_salt) <- u8 1;
+       let db' = Buffer.sub #uint8 #(v db_size) #sLen db (size_incr last_before_salt) ssLen in
+       copy ssLen salt db';
+    
+       mgf_sha256 m1Hash db_size dbMask;
+       xor_bytes db_size db dbMask;
+       
+       let em' = Buffer.sub #uint8 #emLen #(v db_size) em (size 0) db_size in
+       copy db_size db em';
+       let em' = Buffer.sub #uint8 #emLen #(v hLen) em db_size hLen in
+       copy hLen m1Hash em';
        em.(size_decr eemLen) <- u8 0xbc
     )
 		
@@ -107,9 +90,8 @@ val pss_encode:
     em:lbytes emLen -> Stack unit
     (requires (fun h -> live h salt /\ live h msg /\ live h em /\ disjoint msg salt /\ disjoint em msg /\ disjoint em salt))
     (ensures (fun h0 _ h1 -> preserves_live h0 h1 /\ modifies1 em h0 h1))
-
-#reset-options "--z3rlimit 50 --max_fuel 0"
-
+    #reset-options "--z3rlimit 50 --max_fuel 0"
+    [@"c_inline"]
 let pss_encode #sLen #msgLen #emLen msBits ssLen salt mmsgLen msg eemLen em =
     if (msBits =. size 0)
     then begin
@@ -119,68 +101,9 @@ let pss_encode #sLen #msgLen #emLen msBits ssLen salt mmsgLen msg eemLen em =
 	pss_encode_ ssLen salt mmsgLen msg (size_decr eemLen) em' end
     else begin
 	pss_encode_ ssLen salt mmsgLen msg eemLen em;
-	let shift_ = sub #SIZE (size 8) msBits in
-	em.(size 0) <- em.(size 0) &. (shift_right #U8 (u8 0xff) (size_to_uint32 shift_))
+	let shift' = sub #SIZE (size 8) msBits in
+	em.(size 0) <- em.(size 0) &. (shift_right #U8 (u8 0xff) (size_to_uint32 shift'))
     end
-
-
-val pss_verify_in:
-    #sLen:size_nat -> #msgLen:size_nat -> #emLen:size_nat -> #stLen:size_nat ->
-    ssLen:size_t{v ssLen == sLen /\ sLen + v hLen + 8 < max_size_t} ->
-    msBits:size_t{v msBits < 8} ->
-    eemLen:size_t{v eemLen == emLen /\ emLen - sLen - v hLen - 2 >= 0} -> em:lbytes emLen ->
-    mmsgLen:size_t{v mmsgLen == msgLen} -> msg:lbytes msgLen ->
-    pad_size:size_t{v pad_size = emLen - sLen - v hLen - 1} ->
-    db_size:size_t{v db_size = emLen - v hLen - 1} ->
-    m1_size:size_t{v m1_size = 8 + v hLen + sLen} ->
-    sstLen:size_t{v sstLen == stLen /\ stLen = v hLen + v pad_size + v db_size + v m1_size + v hLen} ->
-    st:lbytes stLen -> Stack bool
-    (requires (fun h -> live h em /\ live h msg /\ live h st /\ disjoint em st /\ disjoint st em /\ disjoint st msg))
-    (ensures (fun h0 _ h1 -> preserves_live h0 h1 /\ modifies1 st h0 h1))
-
-#reset-options "--z3rlimit 50 --max_fuel 0 --max_ifuel 0"
-[@ "substitute"]
-let pss_verify_in #sLen #msgLen #emLen #stLen ssLen msBits eemLen em mmsgLen msg pad_size db_size m1_size sstLen st =
-    assume (8 + 2 * v hLen + v hLen * v (blocks db_size hLen) < max_size_t);
-    
-    let mHash = Buffer.sub #uint8 #stLen #(v hLen) st (size 0) hLen in
-    disjoint_sub_lemma1 st msg (size 0) hLen;
-    hash_sha256 mHash mmsgLen msg;
-    
-    let pad2 = Buffer.sub #uint8 #stLen #(v pad_size) st hLen pad_size in
-    pad2.(size_decr pad_size) <- u8 0x01;
-
-    let maskedDB = Buffer.sub #uint8 #emLen #(v db_size) em (size 0) db_size in
-    let m1Hash = Buffer.sub #uint8 #emLen #(v hLen) em db_size hLen in
-    let dbMask = Buffer.sub #uint8 #stLen #(v db_size) st (add #SIZE hLen pad_size) db_size in
-    mgf_sha256 m1Hash db_size dbMask;
-    xor_bytes db_size dbMask maskedDB;
-    
-    (if (msBits >. size 0) then begin
-      let shift_ = sub #SIZE (size 8) msBits in
-      dbMask.(size 0) <- dbMask.(size 0) &. (shift_right #U8 (u8 0xff) (size_to_uint32 shift_)) end);
-
-    //let pad = Buffer.sub #uint8 #(v db_size) #(v pad_size) dbMask (size 0) pad_size in
-    let pad = Buffer.sub #uint8 #stLen #(v pad_size) st (add #SIZE hLen pad_size) pad_size in
-    let salt = Buffer.sub #uint8 #(v db_size) #sLen dbMask pad_size ssLen in
-
-    let m1 = Buffer.sub #uint8 #stLen #(v m1_size) st (add #SIZE (add #SIZE hLen pad_size) db_size) m1_size in
-    let m1Hash' = Buffer.sub #uint8 #stLen #(v hLen) st (add #SIZE (add #SIZE (add #SIZE hLen pad_size) db_size) m1_size) hLen in
-
-    disjoint_sub_lemma2 st (add #SIZE hLen pad_size) pad_size hLen pad_size;
-    let res = 
-	if not (eq_b pad_size pad pad2) then false 
-	else begin	
-	     let m1_ = Buffer.sub #uint8 #(v m1_size) #(v hLen) m1 (size 8) hLen in
-	     copy hLen mHash m1_;
-	     let m1_ = Buffer.sub #uint8 #(v m1_size) #sLen m1 (add #SIZE (size 8) hLen) ssLen in
-	     copy ssLen salt m1_;
-	     hash_sha256 m1Hash' m1_size m1;
-	     disjoint_sub_lemma3 em st db_size hLen (add #SIZE (add #SIZE (add #SIZE hLen pad_size) db_size) m1_size) hLen;
-	     eq_b hLen m1Hash m1Hash'
-	end in
-    res
-
 
 val pss_verify_:
     #sLen:size_nat -> #msgLen:size_nat -> #emLen:size_nat ->
@@ -192,21 +115,57 @@ val pss_verify_:
     msg:lbytes msgLen -> Stack bool
     (requires (fun h -> live h em /\ live h msg /\ disjoint em msg))
     (ensures (fun h0 _ h1 -> preserves_live h0 h1 /\ modifies0 h0 h1))
-
+    #reset-options "--z3rlimit 150 --max_fuel 0 --max_ifuel 0"
+    [@"c_inline"]
 let pss_verify_ #sLen #msgLen #emLen ssLen msBits eemLen em mmsgLen msg =
-    let pad_size = sub #SIZE (sub #SIZE (sub #SIZE eemLen ssLen) hLen) (size 1) in
-    let db_size = sub #SIZE (sub #SIZE eemLen hLen) (size 1) in
-    let m1_size = add #SIZE (add #SIZE (size 8) hLen) ssLen in
+    let pad_size:size_t = sub #SIZE (sub #SIZE (sub #SIZE eemLen ssLen) hLen) (size 1) in
+    let db_size:size_t = sub #SIZE (sub #SIZE eemLen hLen) (size 1) in
+    let m1_size:size_t = add #SIZE (add #SIZE (size 8) hLen) ssLen in
     
-    assume (v hLen + v pad_size + v db_size + v m1_size + v hLen < max_size_t);
+    assume (2 * emLen +  8 + v hLen  < max_size_t);
+    assume (4 + 2 * v hLen + v hLen * v (blocks db_size hLen) < max_size_t);
     let stLen = add #SIZE (add #SIZE (add #SIZE (add #SIZE hLen pad_size) db_size) m1_size) hLen in
     
     alloc #uint8 #bool #(v stLen) stLen (u8 0) [BufItem em; BufItem msg] []
     (fun h0 _ h1 -> True)
     (fun st ->
-	  pss_verify_in #sLen #msgLen #emLen #(v stLen) ssLen msBits eemLen em mmsgLen msg pad_size db_size m1_size stLen st
-    )
+       let mHash = Buffer.sub #uint8 #(v stLen) #(v hLen) st (size 0) hLen in
+       let pad2 = Buffer.sub #uint8 #(v stLen) #(v pad_size) st hLen pad_size in
+       let dbMask = Buffer.sub #uint8 #(v stLen) #(v db_size) st (add #SIZE hLen pad_size) db_size in
+       let m1 = Buffer.sub #uint8 #(v stLen) #(v m1_size) st (add #SIZE (add #SIZE hLen pad_size) db_size) m1_size in
+       let m1Hash' = Buffer.sub #uint8 #(v stLen) #(v hLen) st (add #SIZE (add #SIZE (add #SIZE hLen pad_size) db_size) m1_size) hLen in
+       
+       disjoint_sub_lemma1 st msg (size 0) hLen;
+       hash_sha256 mHash mmsgLen msg;
+       
+       pad2.(size_decr pad_size) <- u8 0x01;
+       let maskedDB = Buffer.sub #uint8 #emLen #(v db_size) em (size 0) db_size in
+       let m1Hash = Buffer.sub #uint8 #emLen #(v hLen) em db_size hLen in
+       mgf_sha256 m1Hash db_size dbMask;
+       xor_bytes db_size dbMask maskedDB;
+    
+       (if (msBits >. size 0) then begin
+	 let shift' = sub #SIZE (size 8) msBits in
+	 dbMask.(size 0) <- dbMask.(size 0) &. (shift_right #U8 (u8 0xff) (size_to_uint32 shift')) end);
 
+       //let pad = Buffer.sub #uint8 #stLen #(v pad_size) st (add #SIZE hLen pad_size) pad_size in
+       let pad = Buffer.sub #uint8 #(v db_size) #(v pad_size) dbMask (size 0) pad_size in
+       let salt = Buffer.sub #uint8 #(v db_size) #sLen dbMask pad_size ssLen in
+
+       assume (disjoint pad pad2);
+       let res =
+	 if not (eq_b pad_size pad pad2) then false
+	 else begin
+	     let m1' = Buffer.sub #uint8 #(v m1_size) #(v hLen) m1 (size 8) hLen in
+	     copy hLen mHash m1';
+	     let m1' = Buffer.sub #uint8 #(v m1_size) #sLen m1 (add #SIZE (size 8) hLen) ssLen in
+	     copy ssLen salt m1';
+	     hash_sha256 m1Hash' m1_size m1;
+	     disjoint_sub_lemma3 em st db_size hLen (add #SIZE (add #SIZE (add #SIZE hLen pad_size) db_size) m1_size) hLen;
+	     eq_b hLen m1Hash m1Hash'
+	end in
+      res
+    )
 
 val pss_verify:
     #sLen:size_nat -> #msgLen:size_nat -> #emLen:size_nat ->
@@ -217,9 +176,8 @@ val pss_verify:
     mmsgLen:size_t{v mmsgLen == msgLen} -> msg:lbytes msgLen -> Stack bool
     (requires (fun h -> live h em /\ live h msg /\ disjoint em msg))
     (ensures (fun h0 _ h1 -> preserves_live h0 h1 /\ modifies0 h0 h1))
-
-#reset-options "--z3rlimit 50 --max_fuel 0 --max_ifuel 0"
-
+    #reset-options "--z3rlimit 50 --max_fuel 0 --max_ifuel 0"
+    [@"c_inline"]
 let pss_verify #sLen #msgLen #emLen ssLen msBits eemLen em mmsgLen msg =
     let h0 = FStar.HyperStack.ST.get() in
     let em_0 = em.(size 0) &. (shift_left #U8 (u8 0xff) (size_to_uint32 msBits)) in
@@ -244,39 +202,47 @@ let pss_verify #sLen #msgLen #emLen ssLen msBits eemLen em mmsgLen msg =
     res
 
 val rsa_sign:
-    #sLen:size_nat -> #msgLen:size_nat ->
-    pow2_i:size_t -> iLen:size_t ->
-    modBits:size_t{0 < v modBits /\ v modBits + 3 < max_size_t} ->
+    #sLen:size_nat -> #msgLen:size_nat -> #nLen:size_nat ->
+    pow2_i:size_t{9 * (1 + nLen) + 4 * v pow2_i < max_size_t /\ (1 + nLen) < v pow2_i} ->
+    iLen:size_t{v iLen < v pow2_i / 2 /\ v iLen + (1 + nLen) = v pow2_i} ->
+    modBits:size_t{0 < v modBits /\ nLen = v (bits_to_bn modBits)} ->
     eBits:size_t{0 < v eBits /\ v eBits <= v modBits} ->
     dBits:size_t{0 < v dBits /\ v dBits <= v modBits} ->
-    pLen:size_t -> qLen:size_t{v (bits_to_bn modBits) + v (bits_to_bn eBits) + v (bits_to_bn dBits) + v pLen + v qLen < max_size_t } ->
-    skey:lbignum (v (bits_to_bn modBits) + v (bits_to_bn eBits) + v (bits_to_bn dBits) + v pLen + v qLen) ->
+    pLen:size_t -> qLen:size_t{nLen + v (bits_to_bn eBits) + v (bits_to_bn dBits) + v pLen + v qLen < max_size_t} ->
+    skey:lbignum (nLen + v (bits_to_bn eBits) + v (bits_to_bn dBits) + v pLen + v qLen) ->
     rBlind:uint64 ->
-    ssLen:size_t{v ssLen == sLen /\ sLen + v hLen + 8 < max_size_t /\ v (blocks modBits (size 8)) - sLen - v hLen - 3 >= 0 } ->
-    salt:lbytes sLen ->
+    ssLen:size_t{v ssLen == sLen /\ sLen + v hLen + 8 < max_size_t /\ v (blocks modBits (size 8)) - sLen - v hLen - 3 >= 0} -> salt:lbytes sLen ->
     mmsgLen:size_t{v mmsgLen == msgLen /\ msgLen < pow2 61} -> msg:lbytes msgLen ->
     sgnt:lbytes (v (blocks modBits (size 8))) -> Stack unit
     (requires (fun h -> live h salt /\ live h msg /\ live h sgnt /\ live h skey /\
 	              disjoint msg salt /\ disjoint msg sgnt /\ disjoint sgnt salt))
     (ensures (fun h0 _ h1 -> preserves_live h0 h1 /\ modifies1 sgnt h0 h1))
 
-#reset-options "--z3rlimit 300 --max_fuel 0 --max_ifuel 0"
-
-let rsa_sign #sLen #msgLen pow2_i iLen modBits eBits dBits pLen qLen skey rBlind ssLen salt mmsgLen msg sgnt =
-    let nLen = bits_to_bn modBits in
-    let eLen = bits_to_bn eBits in
-    let dLen = bits_to_bn dBits in
-    let skeyLen = add #SIZE (add #SIZE (add #SIZE (add #SIZE nLen eLen) dLen) pLen) qLen in
+    #reset-options "--z3rlimit 500 --max_fuel 0 --max_ifuel 0"
+     
+let rsa_sign #sLen #msgLen #nLen pow2_i iLen modBits eBits dBits pLen qLen skey rBlind ssLen salt mmsgLen msg sgnt =
     let k = blocks modBits (size 8) in
     let msBits = (size_decr modBits) %. size 8 in
+
+    //let nLen = bits_to_bn modBits in
+    let nLen = get_size_nat k in
+    let eLen = bits_to_bn eBits in
+    let dLen = bits_to_bn dBits in
+    let skeyLen:size_t = add #SIZE (add #SIZE (add #SIZE (add #SIZE nLen eLen) dLen) pLen) qLen in
     
-    assume (v nLen + v nLen < max_size_t);
-    assume (8 * v (get_size_nat k) < max_size_t);
-    assume (v nLen == v k);
- 
+    let n = Buffer.sub #uint64 #(v skeyLen) #(v nLen) skey (size 0) nLen in
+    let e = Buffer.sub #uint64 #(v skeyLen) #(v eLen) skey nLen eLen in
+    let d = Buffer.sub #uint64 #(v skeyLen) #(v dLen) skey (add #SIZE nLen eLen) dLen in
+    let p = Buffer.sub #uint64 #(v skeyLen) #(v pLen) skey (add #SIZE (add #SIZE nLen eLen) dLen) pLen in
+    let q = Buffer.sub #uint64 #(v skeyLen) #(v qLen) skey (add #SIZE ((add #SIZE (add #SIZE nLen eLen) dLen)) pLen) qLen in
+    
+    assume (2 * v nLen + 2 * (v pLen + v qLen) + 1 < max_size_t);
+    assume (v nLen = v (get_size_nat k));    
+    assume (8 * v nLen < max_size_t);
     let n2Len = add #SIZE nLen nLen in
     let pqLen = add #SIZE pLen qLen in
-    let stLen = add #SIZE n2Len (add #SIZE (add #SIZE pqLen pqLen) (size 1)) in
+    let stLen:size_t = add #SIZE n2Len (add #SIZE (add #SIZE pqLen pqLen) (size 1)) in
+    
     alloc #uint8 #unit #(v k) k (u8 0) [BufItem skey; BufItem msg; BufItem salt] [BufItem sgnt]
     (fun h0 _ h1 -> True)
     (fun em -> 
@@ -285,64 +251,60 @@ let rsa_sign #sLen #msgLen pow2_i iLen modBits eBits dBits pLen qLen skey rBlind
        alloc #uint64 #unit #(v stLen) stLen (u64 0) [BufItem skey; BufItem em] [BufItem sgnt]
 	(fun h0 _ h1 -> True)
 	(fun tmp ->
-	   let n = Buffer.sub #uint64 #(v skeyLen) #(v nLen) skey (size 0) nLen in
-	   let e = Buffer.sub #uint64 #(v skeyLen) #(v eLen) skey nLen eLen in
-	   let d = Buffer.sub #uint64 #(v skeyLen) #(v dLen) skey (add #SIZE nLen eLen) dLen in
-	   let p = Buffer.sub #uint64 #(v skeyLen) #(v pLen) skey (add #SIZE (add #SIZE nLen eLen) dLen) pLen in
-	   let q = Buffer.sub #uint64 #(v skeyLen) #(v qLen) skey (add #SIZE ((add #SIZE (add #SIZE nLen eLen) dLen)) pLen) qLen in
-
 	   let m = Buffer.sub #uint64 #(v stLen) #(v nLen) tmp (size 0) nLen in
 	   let s = Buffer.sub #uint64 #(v stLen) #(v nLen) tmp nLen nLen in
            let phi_n = Buffer.sub #uint64 #(v stLen) #(v pqLen) tmp n2Len pqLen in
 	   let p1 = Buffer.sub #uint64 #(v stLen) #(v pLen) tmp (add #SIZE n2Len pqLen) pLen in
 	   let q1 = Buffer.sub #uint64 #(v stLen) #(v qLen) tmp (add #SIZE (add #SIZE n2Len pqLen) pLen) qLen in
 	   let dLen' = add #SIZE (add #SIZE pLen qLen) (size 1) in
-	   let d' = Buffer.sub #uint64 #(v stLen) #(v dLen') tmp (add #SIZE n2Len pqLen) dLen' in
-	   
+	   let d' = Buffer.sub #uint64 #(v stLen) #(v dLen') tmp (add #SIZE n2Len pqLen) dLen' in admit();
+	   assume (disjoint m em);
 	   text_to_nat k em m;
 	   bn_sub_u64 pLen p (u64 1) p1; // p1 = p - 1
 	   bn_sub_u64 qLen q (u64 1) q1; // q1 = q - 1
 	   bn_mul pLen p1 qLen q1 phi_n; // phi_n = p1 * q1
 	   bn_mul_u64 pqLen phi_n rBlind d'; //d' = phi_n * rBlind
-	   bn_add dLen' d' dLen d d';  //d' = d' + d
+	   bn_add dLen' d' dLen d d'; //d' = d' + d
 	   mod_exp pow2_i iLen modBits nLen n m (mul #SIZE dLen' (size 64)) d' s;
 	   nat_to_text k s sgnt
 	)
     )
 
 val rsa_verify:
-    #sLen:size_nat -> #msgLen:size_nat ->
-    pow2_i:size_t -> iLen:size_t ->
-    modBits:size_t{0 < v modBits /\ v modBits + 3 < max_size_t} ->
-    eBits:size_t{0 < v eBits /\ v eBits <= v modBits /\
-		 v (bits_to_bn modBits) + v (bits_to_bn eBits) < max_size_t} ->
-    pkey:lbignum (v (bits_to_bn modBits) + v (bits_to_bn eBits)) ->
-    ssLen:size_t{v ssLen == sLen /\ sLen + v hLen + 8 < max_size_t} ->
+    #sLen:size_nat -> #msgLen:size_nat -> #nLen:size_nat ->
+    pow2_i:size_t{9 * (1 + nLen) + 4 * v pow2_i < max_size_t /\ (1 + nLen) < v pow2_i} ->
+    iLen:size_t{v iLen < v pow2_i / 2 /\ v iLen + (1 + nLen) = v pow2_i} ->
+    modBits:size_t{0 < v modBits /\ nLen = v (bits_to_bn modBits)} ->
+    eBits:size_t{0 < v eBits /\ v eBits <= v modBits /\ nLen + v (bits_to_bn eBits) < max_size_t} ->
+    pkey:lbignum (nLen + v (bits_to_bn eBits)) ->
+    ssLen:size_t{v ssLen == sLen /\ sLen + v hLen + 8 < max_size_t /\ v (blocks modBits (size 8)) - sLen - v hLen - 3 >= 0} ->
     sgnt:lbytes (v (blocks modBits (size 8))) ->
     mmsgLen:size_t{v mmsgLen == msgLen /\ msgLen < pow2 61} -> msg:lbytes msgLen -> Stack bool
     (requires (fun h -> live h msg /\ live h sgnt /\ live h pkey /\ disjoint msg sgnt))
-    (ensures (fun h0 _ h1 -> preserves_live h0 h1 /\ modifies0 h0 h1))
+    (ensures (fun h0 _ h1 -> preserves_live h0 h1)) // /\ modifies0 h0 h1))
 
-#reset-options "--z3rlimit 50 --max_fuel 0 --max_ifuel 0"
-
-let rsa_verify #sLen #msgLen pow2_i iLen modBits eBits pkey ssLen sgnt mmsgLen msg =
-    let nLen = bits_to_bn modBits in
-    let eLen = bits_to_bn eBits in
-    let pkeyLen = add #SIZE nLen eLen in
+    #reset-options "--z3rlimit 300 --max_fuel 0 --max_ifuel 0"
+    
+let rsa_verify #sLen #msgLen #nLen pow2_i iLen modBits eBits pkey ssLen sgnt mmsgLen msg =
     let k = blocks modBits (size 8) in
     let msBits = (size_decr modBits) %. size 8 in
-    
-    assume (8 * v (get_size_nat k) < max_size_t);
+    //let nLen = bits_to_bn modBits in
+    let nLen = get_size_nat k in
+    let eLen = bits_to_bn eBits in
+    let pkeyLen:size_t = add #SIZE nLen eLen in
+
+    let n = Buffer.sub #uint64 #(v pkeyLen) #(v nLen) pkey (size 0) nLen in
+    let e = Buffer.sub #uint64 #(v pkeyLen) #(v eLen) pkey nLen eLen in
+
+    assume (8 * v nLen < max_size_t);
     assume (v nLen + v nLen < max_size_t);
-    assume (v k - sLen - v hLen - 2 >= 0);
-    assume (v nLen = v k);
     let n2Len:size_t = add #SIZE nLen nLen in
 
     alloc #uint64 #bool #(v n2Len) n2Len (u64 0) [BufItem pkey; BufItem msg; BufItem sgnt] []
     (fun h0 _ h1 -> True)
     (fun tmp ->
 	let s = Buffer.sub #uint64 #(v n2Len) #(v nLen) tmp nLen nLen in
-	(**) disjoint_sub_lemma1 tmp sgnt nLen nLen;
+	disjoint_sub_lemma1 tmp sgnt nLen nLen;
 	text_to_nat k sgnt s;
 
 	alloc #uint8 #bool #(v k) k (u8 0) [BufItem pkey; BufItem msg] [BufItem tmp]
@@ -350,10 +312,7 @@ let rsa_verify #sLen #msgLen pow2_i iLen modBits eBits pkey ssLen sgnt mmsgLen m
 	(fun em ->
             let m = Buffer.sub #uint64 #(v n2Len) #(v nLen) tmp (size 0) nLen in
 	    let s = Buffer.sub #uint64 #(v n2Len) #(v nLen) tmp nLen nLen in
-	
-	    let n = Buffer.sub #uint64 #(v pkeyLen) #(v nLen) pkey (size 0) nLen in
-	    let e = Buffer.sub #uint64 #(v pkeyLen) #(v eLen) pkey nLen eLen in
-
+	    
 	    assume (disjoint s n);
 	    let res = 
 	      if (bn_is_less nLen s nLen n) then begin
@@ -362,6 +321,6 @@ let rsa_verify #sLen #msgLen pow2_i iLen modBits eBits pkey ssLen sgnt mmsgLen m
 		 nat_to_text k m em;
 		 pss_verify #sLen #msgLen #(v k) ssLen msBits k em mmsgLen msg end
 	      else false in
-	    res 
+	    res
        )
     )
